PLC/Relations_aux.v
@@ -8,7 +8,7 @@ Section Reflexive_Transitive_Closure.
   | rt_n_step (y:A) : R x y -> clos_rt_n x y 1
   | rt_n_refl : clos_rt_n x x 0
   | rt_n_trans (y z:A) n1 n2:
-    clos_rt_n x y n1 -> clos_rt_n y z n2 -> clos_rt_n x z (n1 + n2).
+    clos_rt_n x y n1 -> clos_rt_n y z n2 -> clos_rt_n x z (1 + n1 + n2).
 
   Lemma clos_rt_n_rt : forall x y n,
     clos_rt_n x y n -> clos_refl_trans A R x y.
@@ -27,6 +27,23 @@ Section Reflexive_Transitive_Closure.
     exists 0; apply rt_n_refl.
     destruct IHclos_refl_trans1 as [n1 H1].
     destruct IHclos_refl_trans2 as [n2 H2].
-    exists (n1 + n2); eapply rt_n_trans; eauto.
+    exists (1 + n1 + n2); eapply rt_n_trans; eauto.
   Qed.
+
+  Lemma clos_rt_rt_n_equiv : forall x y,
+    clos_refl_trans A R x y <-> exists n, clos_rt_n x y n.
+  Proof.
+    intros x y.
+    split; intro.
+    eauto using clos_rt_rt_n.
+    destruct H; eauto using clos_rt_n_rt.
+  Qed.
+
+  Lemma clos_rt_n_zero : forall x y,
+    clos_rt_n x y 0 -> x = y.
+  Proof.
+    intros x y H; inversion H.
+    reflexivity.
+  Qed.
+
 End Reflexive_Transitive_Closure.
